Source/DafnyCore/Verifier/Translator.ClassMembers.cs
@@ -1098,8 +1098,7 @@ namespace Microsoft.Dafny {
       }
 
       // useViaContext: fh < FunctionContextHeight
-      ModuleDefinition mod = f.EnclosingClass.EnclosingModuleDefinition;
-      Boogie.Expr useViaContext = Boogie.Expr.Lt(Boogie.Expr.Literal(mod.CallGraph.GetSCCRepresentativePredecessorCount(f)), etran.FunctionContextHeight());
+      Boogie.Expr useViaContext = Boogie.Expr.Lt(Boogie.Expr.Literal(forModule.CallGraph.GetSCCRepresentativePredecessorCount(f)), etran.FunctionContextHeight());
 
       // useViaCanCall: C.F#canCall(args)
       Bpl.IdentifierExpr canCallFuncID = new Bpl.IdentifierExpr(overridingFunction.tok, overridingFunction.FullSanitizedName + "#canCall", Bpl.Type.Bool);
@@ -1204,13 +1203,11 @@ namespace Microsoft.Dafny {
         builder.Add(TrAssumeCmd(m.tok, etran.TrExpr(en.E)));
       }
       //generating trait post-conditions with class variables
+      FunctionCallSubstituter sub = null;
       foreach (var en in m.OverriddenMethod.Ens) {
-        Expression postcond = Substitute(en.E, null, substMap, typeMap);
-        bool splitHappened;  // we actually don't care
-        foreach (var s in TrSplitExpr(postcond, etran, false, out splitHappened)) {
-          if (s.IsChecked) {
-            builder.Add(Assert(m.tok, s.E, new PODesc.EnsuresStronger()));
-          }
+        sub ??= new FunctionCallSubstituter(substMap, typeMap, (TraitDecl)m.OverriddenMethod.EnclosingClass, (ClassDecl)m.EnclosingClass);
+        foreach (var s in TrSplitExpr(sub.Substitute(en.E), etran, false, out _).Where(s => s.IsChecked)) {
+          builder.Add(Assert(m.tok, s.E, new PODesc.EnsuresStronger()));
         }
       }
     }
@@ -1223,18 +1220,14 @@ namespace Microsoft.Dafny {
       Contract.Requires(etran != null);
       Contract.Requires(substMap != null);
       //generating trait pre-conditions with class variables
+      FunctionCallSubstituter sub = null;
       foreach (var req in m.OverriddenMethod.Req) {
-        Expression precond = Substitute(req.E, null, substMap, typeMap);
-        builder.Add(TrAssumeCmd(m.tok, etran.TrExpr(precond)));
+        sub ??= new FunctionCallSubstituter(substMap, typeMap, (TraitDecl)m.OverriddenMethod.EnclosingClass, (ClassDecl)m.EnclosingClass);
+        builder.Add(TrAssumeCmd(m.tok, etran.TrExpr(sub.Substitute(req.E))));
       }
       //generating class pre-conditions
-      foreach (var req in m.Req) {
-        bool splitHappened;  // we actually don't care
-        foreach (var s in TrSplitExpr(req.E, etran, false, out splitHappened)) {
-          if (s.IsChecked) {
-            builder.Add(Assert(m.tok, s.E, new PODesc.RequiresWeaker()));
-          }
-        }
+      foreach (var s in m.Req.SelectMany(req => TrSplitExpr(req.E, etran, false, out _).Where(s => s.IsChecked))) {
+        builder.Add(Assert(m.tok, s.E, new PODesc.RequiresWeaker()));
       }
     }
 
@@ -1393,7 +1386,7 @@ namespace Microsoft.Dafny {
       // FREE PRECONDITIONS
       if (kind == MethodTranslationKind.SpecWellformedness || kind == MethodTranslationKind.Implementation || kind == MethodTranslationKind.OverrideCheck) {  // the other cases have no need for a free precondition
         // free requires mh == ModuleContextHeight && fh == FunctionContextHeight;
-        req.Add(Requires(m.tok, true, etran.HeightContext(kind == MethodTranslationKind.OverrideCheck ? m.OverriddenMethod : m), null, null));
+        req.Add(Requires(m.tok, true, etran.HeightContext(m), null, null));
         if (m is TwoStateLemma) {
           // free requires prevHeap == Heap && HeapSucc(prevHeap, currHeap) && IsHeap(currHeap)
           var a0 = Boogie.Expr.Eq(prevHeap, ordinaryEtran.HeapExpr);
